Plfl.lean
@@ -4,3 +4,4 @@ import Plfl.DeBruijn
 import Plfl.More
 import Plfl.More.DoubleSubst
 import Plfl.More.Bisimulation
+import Plfl.Inference
